src/quotient/src/selftest.sml
@@ -1,5 +1,6 @@
 open HolKernel Parse boolLib numLib quotient BasicProvers
 
+val _ = print "Attempting quotient where reln has symbolic name\n"
 val _ = temp_remove_termtok {term_name = "<=>", tok = "<=>"}
 val _ = hide "<=>"
 val eq_def = new_definition("eq_def", ``<=> n m = (n MOD 3 = m MOD 3)``);
@@ -9,5 +10,19 @@ val eq_equiv = prove(``!n m. <=> n m = (<=> n = <=> m)``,
 
 val _ = define_quotient_type "mod3" "abs_mod3" "rep_mod3" eq_equiv
 
+open bossLib
+val _ = Hol_datatype `foo = C1 | C2`
 
+fun mk_def t = let
+  val s = "l" ^ term_to_string t
+in
+  {def_name = s ^ "_def", fixity = Prefix, fname = s, func = t}
+end
+
+val thms = define_equivalence_type {
+             defs = map mk_def [``C1``, ``C2``],
+             equiv = identity_equiv ``:foo``,
+             name = "lfoo",
+             old_thms = [],
+             welldefs = []}
 
