examples/computability/lambda/recsetsScript.sml
@@ -4,8 +4,9 @@ val _ = new_theory "recsets"
 
 open recfunsTheory reductionEval
 open binderLib
-
-val _ = set_trace "Unicode" 1
+open stepsTheory
+open churchlistTheory churchDBTheory
+open normal_orderTheory
 
 fun Store_thm(trip as (n,t,tac)) = store_thm trip before export_rewrites [n]
 
@@ -18,14 +19,14 @@ val empty_recursive = Store_thm(
   ``recursive {}``,
   SRW_TAC [][recursive_def, Phi_def] THEN
   Q.EXISTS_TAC `dBnum (fromTerm (LAM v (church 0)))` THEN
-  SIMP_TAC (bsrw_ss()) [normal_orderTheory.bnf_bnf_of]);
+  SIMP_TAC (bsrw_ss()) [bnf_bnf_of]);
 
 val univ_recursive = Store_thm(
   "univ_recursive",
   ``recursive UNIV``,
   SRW_TAC [][recursive_def, Phi_def] THEN
   Q.EXISTS_TAC `dBnum (fromTerm (LAM v (church 1)))` THEN
-  SIMP_TAC (bsrw_ss()) [normal_orderTheory.bnf_bnf_of]);
+  SIMP_TAC (bsrw_ss()) [bnf_bnf_of]);
 
 val union_recursive_I = Store_thm(
   "union_recursive_I",
@@ -48,7 +49,7 @@ val union_recursive_I = Store_thm(
   Cases_on `n ∈ s₁` THEN Cases_on `n ∈ s₂` THEN
   ASM_SIMP_TAC (bsrw_ss()) [churchboolTheory.cor_behaviour,
                             churchboolTheory.cB_behaviour,
-                            normal_orderTheory.bnf_bnf_of]);
+                            bnf_bnf_of]);
 
 val inter_recursive_I = Store_thm(
   "inter_recursive_I",
@@ -64,7 +65,7 @@ val inter_recursive_I = Store_thm(
   IMP_RES_TAC PhiSOME_UM_I THEN
   ASM_SIMP_TAC (bsrw_ss()) [churchnumTheory.cnpair_behaviour,
                             churchnumTheory.cmult_behaviour,
-                            normal_orderTheory.bnf_bnf_of] THEN
+                            bnf_bnf_of] THEN
   Cases_on `n ∈ s₁` THEN SRW_TAC [][]);
 
 val compl_recursive_I = store_thm(
@@ -81,7 +82,7 @@ val compl_recursive_I = store_thm(
   IMP_RES_TAC PhiSOME_UM_I THEN
   ASM_SIMP_TAC (bsrw_ss()) [churchnumTheory.cnpair_behaviour,
                             churchnumTheory.cminus_behaviour,
-                            normal_orderTheory.bnf_bnf_of] THEN
+                            bnf_bnf_of] THEN
   Cases_on `n ∈ s` THEN SRW_TAC [][]);
 
 val compl_recursive = Store_thm(
@@ -110,9 +111,343 @@ val finite_recursive = Store_thm(
                             churchboolTheory.cor_behaviour] THEN
   Cases_on `n = e` THEN
   ASM_SIMP_TAC (bsrw_ss()) [churchboolTheory.cB_behaviour,
-                            normal_orderTheory.bnf_bnf_of] THEN
+                            bnf_bnf_of] THEN
   Cases_on `n ∈ s` THEN
   ASM_SIMP_TAC (bsrw_ss()) [churchboolTheory.cB_behaviour,
-                            normal_orderTheory.bnf_bnf_of]);
+                            bnf_bnf_of]);
+
+(* an r.e. set is one that can be enumerated.  In this world, I take enumerable
+   to mean there exists a function that returns values at successive indices.
+*)
+val re_def = Define`
+  re s = ∃Mi. ∀e. e ∈ s ⇔ ∃j. Phi Mi j = SOME e
+`;
+
+(* if a set s is r.e., then there is a machine that terminates on only those
+   elements of the set (and fails to terminate on non-members)
+
+   Say the machine we have that enumerates s is Mi.  Then we want one that
+   will correctly terminate on element e of s.
+   For increasing n, construct the list of n elements corresponding to
+   evaluating [Mi 0, Mi 1, Mi 2, ... Mi n] for n steps.  For all the bnfs in
+   this list, see if one of them is equal to e.  If so, terminate.
+*)
+val enum2semibody_def = Define`
+  enum2semibody Mi e loop n j =
+    LAM loop (LAM n
+      (cmem @@ e
+            @@ (cmap @@ cforce_num
+                     @@ (cfilter
+                           @@ cbnf
+                           @@ (ctabulate
+                                 @@ (csuc @@ VAR n)
+                                 @@ (LAM j
+                                       (csteps
+                                          @@ VAR n
+                                          @@ (cdAPP
+                                                @@ (cnumdB @@ church Mi)
+                                                @@ (cchurch @@ VAR j)))))))
+            @@ church 0
+            @@ (VAR loop @@ (csuc @@ VAR n))))
+`;
+
+val enum2semi_def = Define`
+  enum2semi Mi e =
+    let loop = NEW (FV e) in
+    let n = NEW ({loop} ∪ FV e) in
+    let j = NEW {n}
+    in
+       enum2semibody Mi e loop n j
+`;
+
+val FV_enum2semi = Store_thm(
+  "FV_enum2semi",
+  ``FV (enum2semi n t) = FV t``,
+  SRW_TAC [][enum2semi_def, LET_THM, pred_setTheory.EXTENSION,
+             enum2semibody_def] THEN
+  binderLib.NEW_ELIM_TAC THEN REPEAT GEN_TAC THEN
+  binderLib.NEW_ELIM_TAC THEN SRW_TAC [][] THEN
+  METIS_TAC []);
+
+val FV_enum2semibody = Store_thm(
+  "FV_enum2semibody",
+  ``FV (enum2semibody n t x y z) = FV t DELETE x DELETE y``,
+  SRW_TAC [][enum2semibody_def, pred_setTheory.EXTENSION] THEN
+  METIS_TAC []);
+
+val enum2semi_fresh = prove(
+  ``loop ∉ FV e ∧ n ≠ loop ∧ n ∉ FV e ∧ j ≠ n ⇒
+     (enum2semi Mi e = enum2semibody Mi e loop n j)``,
+  SRW_TAC [][enum2semi_def, LET_THM] THEN
+  binderLib.NEW_ELIM_TAC THEN REPEAT STRIP_TAC THEN
+  binderLib.NEW_ELIM_TAC THEN REPEAT STRIP_TAC THEN
+  binderLib.NEW_ELIM_TAC THEN REPEAT STRIP_TAC THEN
+  SRW_TAC [][enum2semibody_def, termTheory.LAM_eq_thm,
+             termTheory.tpm_fresh] THEN
+  Cases_on `loop = v` THEN SRW_TAC [][] THEN1
+    (SRW_TAC [][basic_swapTheory.swapstr_def] THEN METIS_TAC []) THEN
+  Cases_on `v = n` THEN SRW_TAC [][] THEN
+  Cases_on `loop = n` THEN SRW_TAC [][] THENL [
+    Cases_on `loop = j` THEN SRW_TAC [][] THEN
+    SRW_TAC [][basic_swapTheory.swapstr_def, termTheory.tpm_fresh] THEN
+    METIS_TAC [],
+
+    Cases_on `loop = j` THEN SRW_TAC [][] THEN1
+      (SRW_TAC [][basic_swapTheory.swapstr_def, termTheory.tpm_fresh] THEN
+       METIS_TAC []) THEN
+    Cases_on `v = j` THEN SRW_TAC [][] THEN
+    SRW_TAC [][basic_swapTheory.swapstr_def, termTheory.tpm_fresh] THEN
+    METIS_TAC []
+  ]);
+
+val enum2semi_SUB = store_thm(
+  "enum2semi_SUB",
+  ``[N/v] (enum2semi n t) = enum2semi n ([N/v]t)``,
+  Q_TAC (NEW_TAC "loop") `FV N ∪ {v} ∪ FV t` THEN
+  Q_TAC (NEW_TAC "m") `FV N ∪ {v; loop} ∪ FV t` THEN
+  Q_TAC (NEW_TAC "j") `FV N ∪ {v;m}` THEN
+  `enum2semi n t = enum2semibody n t loop m j`
+     by METIS_TAC [enum2semi_fresh] THEN
+  `enum2semi n ([N/v]t) = enum2semibody n ([N/v]t) loop m j`
+     by (MATCH_MP_TAC enum2semi_fresh THEN
+         SRW_TAC [][chap2Theory.NOT_IN_FV_SUB]) THEN
+  SRW_TAC [][enum2semibody_def, termTheory.lemma14b]);
+
+val freshlemma = prove(
+  ``NEW (FV e) ∉ FV e ∧ NEW (FV e ∪ {NEW (FV e)}) ≠ NEW (FV e) ∧
+    NEW (FV e ∪ {NEW (FV e)}) ∉ FV e ∧
+    NEW {NEW (FV e ∪ {NEW (FV e)})} ≠ NEW (FV e ∪ {NEW (FV e)})``,
+  binderLib.NEW_ELIM_TAC THEN NTAC 2 STRIP_TAC THEN
+  binderLib.NEW_ELIM_TAC THEN NTAC 2 STRIP_TAC THEN
+  binderLib.NEW_ELIM_TAC);
+
+val enum2semi_eqn =
+    enum2semi_fresh
+      |> REWRITE_RULE [enum2semibody_def]
+      |> UNDISCH
+      |> brackabs.brackabs_equiv
+          (CONJUNCTS
+               (ASSUME ``loop ∉ FV e ∧ n ≠ loop ∧ n ∉ FV e ∧ j ≠ n``))
+      |> DISCH_ALL
+      |> Q.INST [`j` |-> `NEW {n}`]
+      |> Q.INST [`loop` |-> `NEW (FV e)`, `n` |-> `NEW (FV e ∪ {NEW (FV e)})`]
+      |> C MP freshlemma
+
+val MEM_GENLIST = prove(
+  ``MEM e (GENLIST f n) = ∃i. i < n ∧ (e = f i)``,
+  Q.ID_SPEC_TAC `f` THEN
+  Induct_on `n` THEN1 SRW_TAC [][rich_listTheory.GENLIST] THEN
+  SRW_TAC [][GENLIST_ALT, EQ_IMP_THM] THENL [
+    Cases_on `e = f 0` THENL [
+      Q.EXISTS_TAC `0` THEN SRW_TAC [][],
+      FULL_SIMP_TAC (srw_ss()) [] THEN Q.EXISTS_TAC `SUC i` THEN
+      SRW_TAC [][]
+    ],
+    `∃m. i = SUC m` by METIS_TAC [TypeBase.nchotomy_of ``:num``] THEN
+    Q.EXISTS_TAC `m` THEN SRW_TAC [ARITH_ss][]
+  ]);
+
+val EXISTS_FILTER = store_thm(
+  "EXISTS_FILTER",
+  ``EXISTS P (FILTER Q l) = EXISTS (λe. Q e ∧ P e) l``,
+  Induct_on `l` THEN SRW_TAC [][]);
+
+val EXISTS_GENLIST = prove(
+  ``∀n f. EXISTS P (GENLIST f n) = ∃i. i < n ∧ P (f i)``,
+  Induct THEN1 SRW_TAC [][rich_listTheory.GENLIST] THEN
+  SRW_TAC [][GENLIST_ALT, EQ_IMP_THM] THENL [
+    Q.EXISTS_TAC `0` THEN SRW_TAC [][],
+    Q.EXISTS_TAC `SUC i` THEN SRW_TAC [][],
+    Cases_on `i` THEN SRW_TAC [][] THEN
+    DISJ2_TAC THEN Q.EXISTS_TAC `n'` THEN SRW_TAC [ARITH_ss][]
+  ]);
+
+
+
+val re_semirecursive1 = prove(
+  ``re s ⇒ ∃N. ∀e. e ∈ s ⇔ ∃m. Phi N e = SOME m``,
+  SRW_TAC [][re_def] THEN
+  Q.EXISTS_TAC
+    `dBnum (fromTerm
+              (LAM "e" (chap2$Y @@ enum2semi Mi (VAR "e") @@ church 0)))` THEN
+  SRW_TAC [][Phi_def, EQ_IMP_THM] THENL [
+    SIMP_TAC (bsrw_ss()) [churchDBTheory.cnumdB_behaviour,
+                          Once chap2Theory.lameq_Y, enum2semi_SUB] THEN
+    `toTerm (numdB Mi) @@ church j -n->* z ∧ bnf z`
+       by METIS_TAC [bnf_of_SOME] THEN
+    `∃n. steps n (toTerm (numdB Mi) @@ church j) = z`
+       by METIS_TAC [stepsTheory.bnf_steps] THEN
+    Q.MATCH_ABBREV_TAC
+      `∃r. bnf_of (E @@ (chap2$Y @@ E) @@ church 0) = SOME r` THEN
+    Q_TAC SUFF_TAC `∀st. st ≤ MAX (j + 1) n ⇒
+                         E @@ (chap2$Y @@ E) @@ church st == church 0`
+          THEN1 (DISCH_THEN (Q.SPEC_THEN `0` MP_TAC) THEN
+                 SIMP_TAC (bsrw_ss()) [bnf_bnf_of]) THEN
+    Q_TAC SUFF_TAC
+          `∀m st. (m = MAX (j + 1) n - st) ∧
+                  st ≤ MAX (j + 1) n ⇒
+                  E @@ (chap2$Y @@ E) @@ church st == church 0`
+          THEN1 METIS_TAC [] THEN
+    Induct THEN REPEAT STRIP_TAC THENL [
+      `st = MAX (j + 1) n` by DECIDE_TAC THEN
+      POP_ASSUM SUBST_ALL_TAC THEN
+      SIMP_TAC (bsrw_ss()) [Abbr`E`, enum2semi_eqn] THEN
+      FULL_SIMP_TAC (srw_ss()) [] THEN
+      ASM_SIMP_TAC (bsrw_ss() ++ boolSimps.DNF_ss)
+                   [ctabulate_cvlist, Cong cvlist_genlist_cong,
+                    churchnumTheory.csuc_behaviour,
+                    cchurch_behaviour, cnumdB_behaviour,
+                    cdAPP_behaviour, csteps_behaviour,
+                    cfilter_cvlist, MEM_GENLIST, cbnf_behaviour,
+                    cmap_cvlist, cmem_cvlist, listTheory.MEM_MAP,
+                    listTheory.MEM_FILTER, cforce_num_behaviour] THEN
+      ASM_SIMP_TAC (srw_ss()) [listTheory.EXISTS_MAP,
+                               EXISTS_FILTER, EXISTS_GENLIST] THEN
+      Q.MATCH_ABBREV_TAC `cB P @@ church 0 @@ X == church 0` THEN
+      Q_TAC SUFF_TAC `P` THEN1
+        SIMP_TAC (bsrw_ss()) [churchboolTheory.cB_behaviour] THEN
+      markerLib.UNABBREV_ALL_TAC THEN
+      Q.EXISTS_TAC `j` THEN
+      SIMP_TAC (bsrw_ss()) [cforce_num_behaviour,
+                            churchnumTheory.ceqnat_behaviour,
+                            cbnf_behaviour] THEN
+      `steps (MAX (j + 1) n) (toTerm (numdB Mi) @@ church j) = z`
+         by (SRW_TAC [][] THEN Cases_on `MAX (j + 1) n = n`
+               THEN1 SRW_TAC [][] THEN
+             MATCH_MP_TAC bnf_steps_upwards_closed THEN
+             FULL_SIMP_TAC (srw_ss() ++ ARITH_ss)
+                           [arithmeticTheory.MAX_DEF]) THEN
+      SRW_TAC [ARITH_ss][arithmeticTheory.MAX_DEF],
+
+      `st < MAX (j + 1) n` by DECIDE_TAC THEN
+      SIMP_TAC (bsrw_ss()) [Abbr`E`, Once enum2semi_eqn] THEN
+      ASM_SIMP_TAC (bsrw_ss() ++ boolSimps.DNF_ss)
+                   [ctabulate_cvlist, Cong cvlist_genlist_cong,
+                    churchnumTheory.csuc_behaviour,
+                    cchurch_behaviour, cnumdB_behaviour,
+                    cdAPP_behaviour, csteps_behaviour,
+                    cfilter_cvlist, MEM_GENLIST, cbnf_behaviour,
+                    cmap_cvlist, cmem_cvlist, listTheory.MEM_MAP,
+                    listTheory.MEM_FILTER, cforce_num_behaviour] THEN
+      ASM_SIMP_TAC (srw_ss()) [listTheory.EXISTS_MAP,
+                               EXISTS_FILTER, EXISTS_GENLIST] THEN
+      Q.ABBREV_TAC `MX = MAX (j + 1) n`  THEN
+      FIRST_X_ASSUM (Q.SPEC_THEN `SUC st` MP_TAC) THEN
+      ASM_SIMP_TAC (srw_ss() ++ ARITH_ss) [] THEN
+      STRIP_TAC THEN
+      ASM_SIMP_TAC (bsrw_ss()) [Once chap2Theory.lameq_Y] THEN
+      Q.MATCH_ABBREV_TAC `cB P @@ X @@ X == X` THEN
+      Cases_on `P` THEN
+      ASM_SIMP_TAC (bsrw_ss()) [churchboolTheory.cB_behaviour]
+    ],
+
+    (* other direction: that if our enum2semi function does terminate on an
+       x, then x does indeed appear in the enumeration
+    *)
+    FULL_SIMP_TAC (bsrw_ss())
+                  [enum2semi_SUB,
+                   Once (MATCH_MP relationTheory.RTC_SINGLE
+                                  head_reductionTheory.whY1),
+                   Once (MATCH_MP relationTheory.RTC_SINGLE
+                                  head_reductionTheory.whY2)] THEN
+    FULL_SIMP_TAC (bsrw_ss()) [bnf_steps] THEN
+    NTAC 2 (POP_ASSUM MP_TAC) THEN POP_ASSUM (K ALL_TAC) THEN
+    Q.MATCH_ABBREV_TAC `(steps n (TT @@ church 0) = z) ⇒ bnf z ⇒ Concl` THEN
+    Q_TAC SUFF_TAC
+          `∀n t m. (t == church m) ⇒ (steps n (TT @@ t) = z) ∧ bnf z ⇒
+                   Concl` THEN1 METIS_TAC [chap2Theory.lameq_refl] THEN
+    markerLib.UNABBREV_ALL_TAC THEN
+    completeInduct_on `n` THEN
+    MAP_EVERY Q.X_GEN_TAC [`t`,`m`] THEN STRIP_TAC THEN
+    `lp ∉ FV (church e)` by SRW_TAC [][] THEN
+    Q_TAC (NEW_TAC "nm") `{lp}` THEN
+    Q_TAC (NEW_TAC "jm") `{nm}` THEN
+    `enum2semi Mi (church e) = enum2semibody Mi (church e) lp nm jm`
+       by (MATCH_MP_TAC enum2semi_fresh THEN SRW_TAC [][]) THEN
+    `(n = 0) ∨ (∃n0. n = SUC n0)`
+       by METIS_TAC [TypeBase.nchotomy_of ``:num``]
+       THEN1 (SRW_TAC [][enum2semibody_def] THEN
+              FULL_SIMP_TAC (srw_ss()) []) THEN
+    ASM_SIMP_TAC (srw_ss()) [Once enum2semibody_def, noreduct_thm,
+                             termTheory.lemma14b] THEN
+    `(n0 = 0) ∨ (∃n1. n0 = SUC n1)`
+       by METIS_TAC [TypeBase.nchotomy_of ``:num``]
+       THEN1 (SRW_TAC [][] THEN FULL_SIMP_TAC (srw_ss()) []) THEN
+    ASM_SIMP_TAC (srw_ss()) [noreduct_thm, termTheory.lemma14b] THEN
+    Q.MATCH_ABBREV_TAC
+      `(steps n1 (BoolTerm @@ church 0 @@ Loop) = z) ∧ bnf z ⇒ Concl` THEN
+    `∃b. BoolTerm == cB b`
+       by (SIMP_TAC (bsrw_ss()) [Abbr`BoolTerm`] THEN
+           ASM_SIMP_TAC (bsrw_ss() ++ boolSimps.DNF_ss)
+                        [ctabulate_cvlist, Cong cvlist_genlist_cong,
+                         churchnumTheory.csuc_behaviour,
+                         cchurch_behaviour, cnumdB_behaviour,
+                         cdAPP_behaviour, csteps_behaviour,
+                         cfilter_cvlist, MEM_GENLIST, cbnf_behaviour,
+                         cmap_cvlist, cmem_cvlist, listTheory.MEM_MAP,
+                         listTheory.MEM_FILTER, cforce_num_behaviour]) THEN
+    Cases_on `b` THENL [
+      DISCH_THEN (K ALL_TAC) THEN
+      Q.UNABBREV_TAC `Concl` THEN
+      POP_ASSUM MP_TAC THEN
+      SIMP_TAC (bsrw_ss()) [Abbr`BoolTerm`] THEN
+      ASM_SIMP_TAC (bsrw_ss() ++ boolSimps.DNF_ss)
+                   [ctabulate_cvlist, Cong cvlist_genlist_cong,
+                    churchnumTheory.csuc_behaviour,
+                    cchurch_behaviour, cnumdB_behaviour,
+                    cdAPP_behaviour, csteps_behaviour,
+                    cfilter_cvlist, MEM_GENLIST, cbnf_behaviour,
+                    cmap_cvlist, cmem_cvlist, listTheory.MEM_MAP,
+                    listTheory.MEM_FILTER, cforce_num_behaviour] THEN
+      SIMP_TAC (bsrw_ss()) [listTheory.EXISTS_MAP, EXISTS_FILTER,
+                            EXISTS_GENLIST,
+                            cchurch_behaviour, cdAPP_behaviour,
+                            csteps_behaviour, cbnf_behaviour,
+                            cforce_num_behaviour,
+                            churchnumTheory.ceqnat_behaviour] THEN
+      METIS_TAC [],
+
+      Q.RM_ABBREV_TAC `BoolTerm` THEN
+      IMP_RES_TAC churchboolTheory.whead_tests THEN
+      `BoolTerm @@ church 0 @@ Loop -n->* Loop` by METIS_TAC [whstar_nstar] THEN
+      `∃n2. Loop = steps n2 (BoolTerm @@ church 0 @@ Loop)`
+         by METIS_TAC [nstar_steps] THEN
+      `¬bnf Loop` by (SRW_TAC [][Abbr`Loop`, chap2Theory.Yf_def] THEN
+                      SRW_TAC [][]) THEN
+      REPEAT STRIP_TAC THEN
+      `n2 < n1` by METIS_TAC [DECIDE ``n:num < m ∨ (n = m) ∨ m < n``,
+                              bnf_steps_upwards_closed] THEN
+      `∃rest. n1 = rest + n2` by (Q.EXISTS_TAC `n1 - n2` THEN DECIDE_TAC) THEN
+      FULL_SIMP_TAC (srw_ss()) [steps_plus] THEN
+      `steps rest Loop = z` by METIS_TAC [] THEN
+      `∃r1. rest = SUC r1`
+         by METIS_TAC [TypeBase.nchotomy_of ``:num``, steps_def] THEN
+      Q.ABBREV_TAC `EE = enum2semibody Mi (church e) lp nm jm` THEN
+      `Loop -n-> EE @@ Yf EE @@ (csuc @@ t)`
+         by SRW_TAC [][head_reductionTheory.whY2, Abbr`Loop`, whead_normorder,
+                       head_reductionTheory.weak_head_rules] THEN
+      `noreduct Loop = SOME (EE @@ Yf EE @@ (csuc @@ t))`
+         by FULL_SIMP_TAC (srw_ss()) [noreduct_characterisation] THEN
+      `steps r1 (EE @@ Yf EE @@ (csuc @@ t)) = z`
+         by FULL_SIMP_TAC (srw_ss()) [ASSUME ``¬bnf Loop``] THEN
+      FIRST_X_ASSUM (Q.SPEC_THEN `r1` MP_TAC) THEN
+      ASM_SIMP_TAC (srw_ss() ++ ARITH_ss) [] THEN
+      DISCH_THEN (fn th => MATCH_MP_TAC (REWRITE_RULE [AND_IMP_INTRO] th)) THEN
+      MAP_EVERY Q.EXISTS_TAC [`csuc @@ t`, `SUC m`] THEN
+      ASM_SIMP_TAC (bsrw_ss()) [churchnumTheory.csuc_behaviour]
+    ]
+  ]);
+
+(*
+val recursive_re = store_thm(
+  "recursive_re",
+  ``recursive s ⇒ re s``,
+  SRW_TAC [][recursive_def, re_def] THEN
+  `dBnum (fromTerm
+
+*)
+
+
+
 
 val _ = export_theory ()
