src/HolSmt/HolSmtLib.sml
@@ -7,30 +7,30 @@ structure HolSmtLib :> HolSmtLib = struct
 
   open Abbrev
 
-  fun GENERIC_SMT_TAC solver goal =
-    case solver goal of
-      SolverSpec.SAT NONE =>
-        raise (Feedback.mk_HOL_ERR "HolSmtLib" "GENERIC_SMT_TAC"
-          "solver reports negated term to be 'satisfiable'")
-    | SolverSpec.SAT (SOME _) =>
-        raise (Feedback.mk_HOL_ERR "HolSmtLib" "GENERIC_SMT_TAC"
-          "solver reports negated term to be 'satisfiable' (model returned)")
-    | SolverSpec.UNSAT NONE =>
-        let
-          val thm = Thm.mk_oracle_thm "HolSmtLib" goal
-        in
-          ([], fn _ => thm)
-        end
-    | SolverSpec.UNSAT (SOME thm) =>
-        (* 'thm' should be of the form "A' |- concl", where A' \subseteq A and
+  fun GENERIC_SMT_TAC solver =
+  let
+    val ERR = Feedback.mk_HOL_ERR "HolSmtLib" "GENERIC_SMT_TAC"
+    fun SMT_TAC goal =
+      case solver goal of
+        SolverSpec.SAT NONE =>
+        raise ERR "solver reports negated term to be 'satisfiable'"
+      | SolverSpec.SAT (SOME _) =>
+        raise ERR
+          "solver reports negated term to be 'satisfiable' (model returned)"
+      | SolverSpec.UNSAT NONE =>
+        ([], fn _ => Thm.mk_oracle_thm "HolSmtLib" goal)
+      | SolverSpec.UNSAT (SOME thm) =>
+        (* 'thm' should be of the form "A' |- concl", where A' \subseteq A, and
            (A, concl) is the input goal (cf. SolverSpec.sml) *)
         ([], fn _ => thm)
-    | SolverSpec.UNKNOWN NONE =>
-        raise (Feedback.mk_HOL_ERR "HolSmtLib" "GENERIC_SMT_TAC"
-          "solver reports 'unknown' (solver not installed/problem too hard?)")
-    | SolverSpec.UNKNOWN (SOME message) =>
-        raise (Feedback.mk_HOL_ERR "HolSmtLib" "GENERIC_SMT_TAC"
-          ("solver reports 'unknown' (" ^ message ^ ")"))
+      | SolverSpec.UNKNOWN NONE =>
+        raise ERR
+          "solver reports 'unknown' (solver not installed/problem too hard?)"
+      | SolverSpec.UNKNOWN (SOME message) =>
+        raise ERR ("solver reports 'unknown' (" ^ message ^ ")")
+  in
+    Tactical.THENL (Tactical.REPEAT Tactic.GEN_TAC, [SMT_TAC])
+  end
 
   val YICES_TAC = GENERIC_SMT_TAC Yices.Yices_Oracle
   val CVC3_TAC = GENERIC_SMT_TAC CVC3.CVC3_SMT_Oracle
